Linglib/Studies/Sag2010.lean
@@ -4,7 +4,6 @@ Released under Apache 2.0 license as described in the file LICENSE.
 Authors: Robert Hawkins
 -/
 import Linglib.Syntax.HPSG.Construction
-import Linglib.Studies.Ross1967
 import Linglib.Studies.SagWasowBender2003
 import Linglib.Semantics.Mood.Defs
 
